SkLean/Sn.lean
@@ -12,14 +12,14 @@ import SkLean.Typing
 open SkExpr
 
 inductive Sn : SkExpr → Prop
-  | trivial e : eval_once e = e    → Sn e
-  | hard    e : (Sn ∘ eval_once) e → Sn e
+  | trivial (call : Call) : eval_once call = (.call call) → Sn (.call call)
+  | hard    (call : Call) : (Sn ∘ eval_once) call → Sn (.call call)
 
 /-
 I reuse the [previous lemmas](./SnLc.lean.md) about SN bidirectionality.
 -/
 
-lemma eval_rfl_imp_sn_iff : ∀ e, eval_once e = e → (Sn (eval_once e) ↔ Sn e) := by
+lemma eval_rfl_imp_sn_iff : ∀ (call : Call), eval_once call = (.call call) → (Sn (eval_once call) ↔ Sn (.call call)) := by
   intro e h_eq
   constructor
   rw [h_eq]
@@ -27,55 +27,17 @@ lemma eval_rfl_imp_sn_iff : ∀ e, eval_once e = e → (Sn (eval_once e) ↔ Sn 
   rw [h_eq]
   simp
 
-lemma sn_bidirectional : ∀ (e : SkExpr), Sn (eval_once e) ↔ Sn e := by
+lemma sn_bidirectional : ∀ (call : Call), Sn (eval_once call) ↔ Sn (.call call) := by
   intro e
-  match e with
-    | .var n =>
-      have h : eval_once (.var n) = (.var n) := by
-        unfold eval_once
-        simp
-      apply eval_rfl_imp_sn_iff
-      exact h
-    | .call lhs rhs =>
-      constructor
-      intro h
-      apply Sn.hard
-      exact h
-      intro h
-      cases h
-      case mpr.trivial a =>
-        rw [a]
-        apply Sn.trivial
-        exact a
-      case mpr.hard a =>
-        exact a
-    | .k =>
-      have h : eval_once k = k := by
-        unfold eval_once
-        simp
-      apply eval_rfl_imp_sn_iff
-      exact h
-    | .s =>
-      have h : eval_once s = s := by
-        unfold eval_once
-        simp
-      apply eval_rfl_imp_sn_iff
-      exact h
-    | .fall a b =>
-      have h : eval_once (fall a b) = fall a b := by
-        unfold eval_once
-        simp
-      apply eval_rfl_imp_sn_iff
-      exact h
-    | .prp =>
-      have h : eval_once prp = prp := by
-        unfold eval_once
-        simp
-      apply eval_rfl_imp_sn_iff
-      exact h
-    | .ty n =>
-      have h : eval_once (ty n) = ty n := by
-        unfold eval_once
-        simp
-      apply eval_rfl_imp_sn_iff
-      exact h
+  constructor
+  intro h
+  apply Sn.hard
+  exact h
+  intro h
+  cases h
+  case mpr.trivial a =>
+    rw [a]
+    apply Sn.trivial
+    exact a
+  case mpr.hard a =>
+    exact a
